Made some progress in body_delete
1. Refactor in_tree_****_range so as to use them in both body_lookup and body_delete.
2. Every piece except the call of pushdown_left is proved in body_delete.
3. Proved pure fact delete_sorted.

concurrency/verif_bst_conc_atomic_delete.v
@@ -130,117 +130,142 @@ Proof.
       { contradiction. }
       { Exists g_root gbr k v tb' tbr lockb' ltbr. cancel.
         unfold ltree at 3. entailer!.
-        rewrite later_sepcon. cancel. }
+(*        rewrite later_sepcon. cancel. }
     Exists tb' lockb' tbl ltbl.
     entailer!.
     unfold ltree at 1.
     entailer!. }
+*)
 Admitted.
 
-Definition delete_inv (b: val) (sh: share) (* (lock: val) *) (x: Z) (* (v: val) *) (g_root: gname) gv (inv_names : invG) (Q : mpred) (g:gname) : environ -> mpred :=
-  ( EX np: val, EX r: number * number * option ghost_info, EX g_in :gname, EX lock : val,
-  PROP ( check_key_exist x (fst r) = true )
-  LOCAL (temp _l lock; temp _tgt np; temp _t b; temp _x (vint x); (* temp _value v; *) gvars gv)
-  SEP (lock_inv sh lock (node_lock_inv g np g_in lock);
-  node_lock_inv g np g_in lock;
-(* lock_inv sh lock (sync_inv g_in (node_rep np g )); node_rep np g g_in r; my_half g_in r; *)
-  atomic_shift (λ BST : @tree val, tree_rep2 g g_root BST ) ∅ ⊤
-    (λ (BST : @tree val) (_ : ()),
-       fold_right_sepcon [tree_rep2 g g_root (delete x BST) ]) 
-    (λ _ : (), Q);
-    mem_mgr gv; data_at sh (tptr t_struct_tree_t) np b ;
-(*      !!(field_compatible t_struct_tree_t nil np) && *)
-    field_at sh t_struct_tree_t [StructField _lock] lock np))%assert.
-
-Set Default Timeout 30.
+Definition delete_inv (b: val) (lock: val) (sh: share) (x: Z) (g_root: gname) gv
+           (inv_names : invG) (Q : mpred) (g:gname) : environ -> mpred :=
+  (EX np: val, EX r: number * number * option ghost_info,
+   EX g_in: gname, EX lock_in: val,
+  PROP ( check_key_exist' x (fst r) = true )
+  LOCAL (temp _l lock_in; temp _tgt np; temp _t b; temp _x (vint x); gvars gv)
+  SEP (nodebox_rep g g_root sh lock b; 
+      field_at lsh2 t_struct_tree_t [StructField _lock] lock_in np ;
+      malloc_token Ews tlock lock_in;
+      node_rep np g g_in r; my_half g_in r;
+      |> lock_inv lsh2 lock_in  (node_lock_inv g np g_in lock_in);
+      atomic_shift
+        (λ BST : @tree val, !! sorted_tree BST && tree_rep2 g g_root BST ) ∅ ⊤
+        (λ (BST : @tree val) (_ : ()),
+         fold_right_sepcon [!! sorted_tree (delete x BST) &&
+                            tree_rep2 g g_root (delete x BST) ]) 
+        (λ _: (), Q); mem_mgr gv))%assert.
 
 Lemma body_delete: semax_body Vprog Gprog f_delete delete_spec.
 Proof.
   start_function.
-  unfold nodebox_rep; Intros p.
-  unfold ltree; Intros.
-  forward.
-  forward.
-  forward_call (lockb, sh, node_lock_inv g p g_root lockb). (* acquire(_l); *)
-  setoid_rewrite node_lock_inv_def at 2.
-  Intros rp; destruct rp as (rangep, g_infop).
-  rewrite node_rep_def; Intros tpv; simpl.
-  forward_loop (delete_inv b sh (* lockb *) x g_root gv inv_names Q g).
-  { unfold delete_inv.
-    Exists (p) (rangep, g_infop) (g_root) (lockb).
-    go_lower. entailer!.
-    { admit. }
-    { setoid_rewrite node_lock_inv_def at 2.
-      Exists (rangep, g_infop). cancel.
-      rewrite node_rep_def. Exists tpv; simpl. cancel. }}
-  unfold delete_inv. clear dependent p. Intros p rp g_in lockp.
-  setoid_rewrite node_lock_inv_def at 2. Intros rp'; destruct rp' as (rangep', g_infop').
-  rewrite node_rep_def; Intros tpv'; simpl.
-  forward.
-  forward_if. (* p == NULL *)
-  { forward_call (lockp, lsh2, node_lock_inv_pred g p g_in lockp, node_lock_inv g p g_in lockp).
-    { lock_props.
-      setoid_rewrite node_lock_inv_def at 3. Exists (rangep', g_infop').
-      rewrite node_rep_def. Exists tpv'; simpl.
-      cancel. }
-    forward.
-    { admit. }}
-  { unfold tree_rep_R. if_tac.
-    { contradiction. }
-    { Intros gl gr k v pl pr lockl lockr.
-      forward. (* y = p->key *)
-      forward_if. (* x < y *)
-      { forward.
-        forward.
-        unfold ltree at 1; Intros.
-        forward.
-        forward_call (lockl, lsh1, node_lock_inv g pl gl lockl). (* acquire(_l); *)
-        forward_call (lockp, lsh2, node_lock_inv_pred g p g_in lockp, node_lock_inv g p g_in lockp).
-        { lock_props.
-          setoid_rewrite node_lock_inv_def at 5. Exists (rangep', g_infop').
-          rewrite node_rep_def. Exists tpv'; simpl.
-          unfold tree_rep_R.
-          if_tac.
-          { contradiction. }
-          { Exists (gl) (gr) k v pl pr lockl lockr. cancel.
-            unfold ltree at 1. entailer!.
-            rewrite later_sepcon.
-            cancel. }}
-        unfold delete_inv.
-        Exists (pl) (rangep', g_infop') (g_in) (lockl).
-        go_lower. entailer!.
-        { admit. }
-        admit.
-        (* rewrite t_lock_pred_def at 1. Intros t' tp'.
-        unfold t_lock_pred_base. Exists (t') (tp').
-        entailer!. *) }
-      forward_if. (* y < x *)
-      { admit. (* forward.
-        forward.
-        unfold ltree at 2; Intros.
-        forward.
-        forward_call (lockr, lsh1, t_lock_pred pr lockr). (* acquire(_l); *)
-        forward_call (lockp, lsh2, t_lock_pred_base p lockp, t_lock_pred p lockp).
-        { lock_props.
-          setoid_rewrite t_lock_pred_def at 4. Exists (tvp) (tp).
-          unfold node_rep. rewrite E.
-          Exists (pl) (pr) (lockl) (lockr). unfold ltree at 3.
-          entailer!.
-          rewrite later_sepcon.
-          cancel. }
-        unfold delete_inv.
-        Exists (pr) (lockr).
-        rewrite t_lock_pred_def at 1. Intros t' tp'.
-        unfold t_lock_pred_base. Exists t' tp'.
-        entailer!. *)
-        }
-      { (* else case *)
-        assert_PROP (field_compatible t_struct_tree_t [] p). {
-          entailer!.
-        }
-        forward_call (p, tp, lockp, k, v, lockl, lockr, pl, pr, gv).
-        { unfold ltree. entailer!. }
-        forward. }
-      }
-    }
-Qed.
+  unfold nodebox_rep, ltree. Intros np.
+  forward. (* _tgt = *_t; *)
+  forward. (* _l = (_tgt -> _lock); *)
+  forward_call (lock, sh, node_lock_inv g np g_root lock). (* acquire(_l); *)
+  unfold node_lock_inv at 2. rewrite selflock_eq. Intros.
+  fold (node_lock_inv g np g_root lock). unfold node_lock_inv_pred, sync_inv.
+  Intros rp; destruct rp as (rangep, g_infop). rewrite node_rep_def. Intros tp.
+  forward_loop (delete_inv b lock sh x g_root gv inv_names Q g).
+  - (* current status implies lookup_inv *)
+    unfold delete_inv. Exists np (rangep, g_infop) g_root lock.
+    gather_SEP (atomic_shift _ _ _ _ _) (my_half _ _) (in_tree g _).
+    sep_apply (in_tree_root_range
+                 unit
+                 (λ (BST : tree) (_ : ()),
+                  !! sorted_tree (delete x BST) && tree_rep2 g g_root (delete x BST) *
+                  emp) (λ _ : (), Q) g g_root inv_names rangep g_infop).
+    entailer. cancel. unfold nodebox_rep. Exists np. cancel. unfold ltree. entailer!.
+    rewrite node_rep_def. Exists tp. simpl. cancel.
+  - (* loop body *)
+    clear np H0 rangep g_infop tp. unfold delete_inv. Intros np r g_in lock_in.
+    rewrite node_rep_def. Intros tp.
+    forward. (* _p = (_tgt -> _t); *)
+    forward_if. (* if (_p == (tptr tvoid) (0)) *)
+    + (* then branch *)
+      subst tp. unfold tree_rep_R. simpl. Intros.
+      gather_SEP (atomic_shift _ _ _ _ _) (my_half g_in _) (in_tree g _).
+      viewshift_SEP 0 (Q * (in_tree g g_in * my_half g_in r)). {
+        go_lower. apply sync_commit_gen1. intros t. unfold tree_rep2 at 1. Intros tg.
+        assert_PROP (Ensembles.In _ (find_ghost_set tg g_root) g_in). {
+          sep_apply node_exist_in_tree. entailer!. }
+        sep_apply (ghost_tree_rep_public_half_ramif
+                     _ _ (Neg_Infinity, Pos_Infinity) _ H4). Intros r0.
+      eapply derives_trans; [|apply ghost_seplog.bupd_intro]. Exists r0. cancel.
+      apply imp_andp_adjoint. Intros. subst r0. Exists r.
+      rewrite <- wand_sepcon_adjoint.
+      eapply derives_trans; [|apply ghost_seplog.bupd_intro].
+      Exists tt. entailer. rewrite sepcon_comm. rewrite <- !sepcon_assoc.
+      sep_apply wand_frame_elim. destruct r as [rg r2]. simpl in H1, H0. subst r2.
+      assert (delete x (find_pure_tree tg) = find_pure_tree tg). {
+        apply delete_not_in.
+        apply (range_info_in_tree_not_In _ _ rg (Neg_Infinity, Pos_Infinity)); auto. }
+      rewrite !H1. apply andp_right. 1: apply prop_right; auto.
+      cancel. unfold tree_rep2. Exists tg. entailer!. }
+      forward_call (lock_in, lsh2, node_lock_inv_pred g np g_in lock_in,
+                    node_lock_inv g np g_in lock_in). (* _release2(_l); *)
+      * lock_props. unfold node_lock_inv at 2. rewrite selflock_eq.
+        fold (node_lock_inv g np g_in lock_in). unfold node_lock_inv_pred.
+        unfold sync_inv. Exists r. rewrite node_rep_def. Exists nullval.
+        unfold tree_rep_R. simpl. entailer!.
+      * forward. cancel.
+    + (* else branch *)
+      unfold tree_rep_R. rewrite if_false; auto. Intros ga gb x0 v pa pb locka lockb.
+      forward. (* _y = (_p -> _key); *)
+      forward_if. (* if (_x < _y) { *)
+      * forward. (* _tgt = (_p -> _left); *)
+        forward. (* _l_old = _l; *) unfold ltree at 1. Intros.
+        forward. (* _l = (_tgt -> _lock); *)
+        forward_call (locka, lsh1, (node_lock_inv g pa ga locka)). (* _acquire(_l); *)
+        unfold node_lock_inv at 2. rewrite selflock_eq. Intros.
+        fold (node_lock_inv g pa ga locka). unfold node_lock_inv_pred, sync_inv.
+        Intros a. rewrite node_rep_def. Intros tpa.
+        gather_SEP (atomic_shift _ _ _ _ _) (my_half g_in _)
+                   (in_tree g g_in) (my_half ga a).
+        sep_apply (in_tree_left_range
+                     unit
+                     (λ (BST : tree) (_ : ()),
+                      !! sorted_tree (delete x BST) &&
+                      tree_rep2 g g_root (delete x BST) * emp) (λ _ : (), Q)
+                     x x0 g g_root inv_names v g_in ga gb r a). Intros.
+        forward_call (lock_in, lsh2, node_lock_inv_pred g np g_in lock_in,
+                      node_lock_inv g np g_in lock_in). (* _release2(_l_old); *)
+        -- lock_props. setoid_rewrite node_lock_inv_def at 4. Exists r.
+           rewrite node_rep_def. Exists tp. cancel. unfold tree_rep_R at 2.
+           rewrite if_false; auto. Exists ga gb x0 v pa pb locka lockb. entailer!.
+           unfold ltree. entailer!. rewrite sepcon_comm. rewrite !later_sepcon. cancel.
+        -- unfold delete_inv. Exists pa a ga locka. entailer!.
+           ++ rewrite H8. rewrite andb_true_iff. destruct r. destruct p.
+              simpl fst in *. apply andb_true_iff in H0. destruct H0. simpl.
+              rewrite Z.ltb_lt. now split.
+           ++ rewrite node_rep_def. Exists tpa. cancel.
+      * forward_if. (* if (_y < _x) { *)
+        -- forward. (* _tgt = (_p -> _right); *)
+           forward. (* _l_old__1 = _l; *) unfold ltree at 2. Intros.
+           forward. (* _l = (_tgt -> _lock); *)
+           forward_call (lockb, lsh1, (node_lock_inv g pb gb lockb)).
+           (* _acquire(_l); *)
+           unfold node_lock_inv at 2. rewrite selflock_eq. Intros.
+           fold (node_lock_inv g pb gb lockb). unfold node_lock_inv_pred, sync_inv.
+           Intros a. rewrite node_rep_def. Intros tpb.
+           gather_SEP (atomic_shift _ _ _ _ _) (my_half g_in _)
+                      (in_tree g g_in) (my_half gb a).
+           sep_apply (in_tree_right_range
+                        unit
+                        (λ (BST : tree) (_ : ()),
+                         !! sorted_tree (delete x BST) &&
+                         tree_rep2 g g_root (delete x BST) * emp) (λ _ : (), Q)
+                        x x0 g g_root inv_names v g_in ga gb r a). Intros.
+           forward_call (lock_in, lsh2, node_lock_inv_pred g np g_in lock_in,
+                         node_lock_inv g np g_in lock_in). (* _release2(_l_old__1); *)
+           ++ lock_props. setoid_rewrite node_lock_inv_def at 4. Exists r.
+              rewrite node_rep_def. Exists tp. cancel. unfold tree_rep_R at 2.
+              rewrite if_false; auto. Exists ga gb x0 v pa pb locka lockb. entailer!.
+              unfold ltree. entailer!. rewrite !later_sepcon. cancel.
+           ++ unfold delete_inv. Exists pb a gb lockb. entailer!.
+              ** rewrite H9. rewrite andb_true_iff. destruct r. destruct p.
+                 simpl fst in *. simpl snd in *. apply andb_true_iff in H0.
+                 destruct H0. split; auto. simpl. now rewrite Z.ltb_lt.
+              ** rewrite node_rep_def. Exists tpb. cancel.
+        -- assert (x0 = x) by lia. subst x0. clear H6 H7.
+Abort.
