concurrency/verif_bst_conc_atomic.v
@@ -106,7 +106,52 @@ Inductive sorted_ghost_tree : ghost_tree -> Prop :=
                         
  end.
 
- 
+ Lemma pushdown_left_In: forall (t1 t2: tree) (x: key),
+     In x (pushdown_left t1 t2) -> In x t1 \/ In x t2.
+ Proof.
+   intros. revert t2 H. induction t2; intros; simpl in *; auto. inv H.
+   - right. now apply InRoot.
+   - apply IHt2_1 in H1. destruct H1; [left | right]; auto. now apply InLeft.
+   - right. now apply InRight.
+ Qed.
+
+ Lemma delete_In: forall (x: key) (t: tree) (y: key), In y (delete x t) -> In y t.
+ Proof.
+   intros. revert t H. induction t; intros; simpl in *; auto. destruct (x <? k).
+   - inv H; try ((now apply InLeft) || (now apply InRoot) || (now apply InRight)).
+     apply IHt1 in H1. now apply InLeft.
+   - destruct (k <? x).
+     + inv H; try ((now apply InLeft) || (now apply InRoot) || (now apply InRight)).
+       apply IHt2 in H1. now apply InRight.
+     + apply pushdown_left_In in H. destruct H; [apply InLeft | apply InRight]; easy.
+ Qed.
+
+ Lemma pushdown_left_sorted: forall (t1 t2: tree),
+     sorted_tree t1 -> sorted_tree t2 -> (forall x y, In x t1 -> In y t2 -> x < y) ->
+     sorted_tree (pushdown_left t1 t2).
+ Proof.
+   intros. revert t2 H0 H1. induction t2; intros; simpl in H0 |-* ; auto.
+   inv H0. constructor; auto.
+   - apply IHt2_1; auto. intros. apply H1; auto. now apply InLeft.
+   - intros z ?. apply pushdown_left_In in H0. destruct H0.
+     + apply Z.lt_gt, H1; auto. now apply InRoot.
+     + now specialize (H8 _ H0).
+ Qed.
+
+ Lemma delete_sorted: forall (x: key) (t: tree),
+     sorted_tree t -> sorted_tree (delete x t).
+ Proof.
+   intros. revert t H. induction t; intros; simpl; auto. inv H.
+   destruct (x <? k) eqn: ?.
+   - apply Z.ltb_lt in Heqb. constructor; auto. intros y ?.
+     apply delete_In in H. now apply H6.
+   - apply Z.ltb_ge in Heqb. destruct (k <? x) eqn: ?.
+     + apply Z.ltb_lt in Heqb0. constructor; auto. intros y ?.
+       apply delete_In in H. now apply H7.
+     + apply pushdown_left_sorted; auto. intros y z ? ?.
+       apply H6 in H. apply H7 in H0. lia.
+ Qed.
+
 End TREES.
 
  Lemma  sample_tree_correctness : sorted_tree (T (T (T E 1 1 E) 2 2 (T E 3 3 E)) 4 4 (T E 5 5 E)).
@@ -734,7 +779,7 @@ intros.
 revert dependent r_root.  
 induction t.
 - intros. simpl. inversion H0. auto.
--  intros.  destruct r_root. simpl.  destruct (x <? k) eqn:E1. SearchAbout Z.ltb.
+-  intros.  destruct r_root. simpl.  destruct (x <? k) eqn:E1.
  * inversion H2;subst. apply IHt1. apply H8. intro a. contradiction H3. apply InLeft. apply a.  inversion H0;subst. apply H5.  apply range_inside_range in H5.
    + unfold range_inclusion in H5. destruct r. apply andb_prop in H5. destruct H5. unfold check_key_exist' in H. apply andb_prop in H.
      destruct H. apply less_than_to_less_than_equal in H. assert ( less_than_equal (Finite_Integer k) (Finite_Integer x) = true ).
@@ -772,7 +817,7 @@ induction t.
  - simpl.  intros. destruct r.  Intros ga gb. destruct (x <? k) eqn: IHe. 
     *  simpl.  Exists ga gb. cancel. apply IHt1. intros a. contradiction H0. apply InLeft. apply a. apply H.
     *  destruct (k <? x) eqn: IHe'. simpl. Exists ga gb.  cancel. apply IHt2. intros a. contradiction H0. apply InRight. apply a. apply H. 
-    contradiction H0. SearchAbout Z.ltb. apply Z.ltb_nlt in IHe. apply Z.ltb_nlt in IHe'. assert (k = x). { omega. } apply InRoot. omega.
+    contradiction H0. apply Z.ltb_nlt in IHe. apply Z.ltb_nlt in IHe'. assert (k = x). { omega. } apply InRoot. omega.
 Qed.
  
  Lemma empty_tree_rep: forall g r,  tree_rep g E r = public_half g r.
@@ -1248,16 +1293,19 @@ Program Definition insert_spec :=
 
 Program Definition delete_spec :=
  DECLARE _delete
-  ATOMIC TYPE (rmaps.ConstType (_ * _ * _ * _ * _ * _ * _)) OBJ BST INVS base.empty base.top
-  WITH b: val, x: Z, lockb: val, gv: globals, sh: share, g: gname, g_root: gname
-  PRE  [ _t OF (tptr (tptr t_struct_tree_t)), _x OF tint]
+ ATOMIC TYPE (rmaps.ConstType (_ * _ * _ * _ * _ * _ * _))
+         OBJ BST INVS base.empty base.top
+ WITH b: val, x: Z, lock: val, gv: globals, sh: share, g: gname, g_root: gname
+ PRE  [ _t OF (tptr (tptr t_struct_tree_t)), _x OF tint]
     PROP (Int.min_signed <= x <= Int.max_signed; readable_share sh)
     LOCAL(temp _t b; temp _x (Vint (Int.repr x)); gvars gv)
-    SEP (mem_mgr gv; nodebox_rep g g_root sh lockb b) | (!!(sorted_tree BST) && tree_rep2 g g_root BST)
+    SEP (mem_mgr gv; nodebox_rep g g_root sh lock b) |
+        (!!(sorted_tree BST) && tree_rep2 g g_root BST)
   POST [ Tvoid ]
     PROP ()
     LOCAL ()
-    SEP (mem_mgr gv; nodebox_rep g g_root sh lockb b) | (!!(sorted_tree (delete x BST)) && tree_rep2 g g_root (delete x BST)).
+    SEP (mem_mgr gv; nodebox_rep g g_root sh lock b) |
+        (!!(sorted_tree (delete x BST)) && tree_rep2 g g_root (delete x BST)).
 
 Notation "'ATOMIC' 'TYPE' W 'OBJ' x 'INVS' Ei Eo 'WITH' x1 : t1 , x2 : t2 , x3 : t3 , x4 : t4 , x5 : t5 , x6 : t6 , x7 : t7 , x8 : t8 , x9 : t9 , x10 : t10 , x11 : t11 'PRE'  [ u , .. , v ] 'PROP' ( Px ; .. ; Py ) 'LOCAL' ( Lx ; .. ; Ly ) 'SEP' ( S1x ; .. ; S1y ) '|' S2 'POST' [ tz ] 'PROP' () 'LOCAL' () 'SEP' ( SPx ; .. ; SPy ) '|' ( SQx ; .. ; SQy )" :=
   (mk_funspec (pair (cons u%formals .. (cons v%formals nil) ..) tz) cc_default (atomic_spec_type0 W)
@@ -1742,20 +1790,25 @@ Proof.
       assert (x = k) by lia. subst. now apply InRoot.
 Qed.
 
+Lemma delete_not_in: forall (t: @tree val) x, ~ In x t -> delete x t = t.
+Proof.
+  intros. revert t H. induction t; intros; simpl; auto. destruct (x <? k) eqn: ?.
+  - rewrite IHt1; auto. intro. now apply H, InLeft.
+  - destruct (k <? x) eqn: ?.
+    + rewrite IHt2; auto. intro. now apply H, InRight.
+    + exfalso. apply H. apply Z.ltb_ge in Heqb. apply Z.ltb_ge in Heqb0.
+      assert (x = k) by lia. subst. now apply InRoot.
+Qed.
+
 Lemma in_tree_root_range:
-  ∀ (x : Z) (g g_root : gname) (Q : val → mpred) (inv_names : invG)
-    (p : number * number) (o : option ghost_info),
+  ∀ (B: Type) (b: tree -> B -> mpred) (Q : B → mpred) (g g_root : gname)
+    (inv_names : invG) (p : number * number) (o : option ghost_info),
     (atomic_shift
-      (λ BST : tree, !! sorted_tree BST && tree_rep2 g g_root BST) ∅ ⊤
-      (λ (BST : tree) (ret : val),
-       !! (sorted_tree BST ∧ ret = lookup nullval x BST) && tree_rep2 g g_root BST *
-       emp) Q *
+      (λ BST : tree, !! sorted_tree BST && tree_rep2 g g_root BST) ∅ ⊤ b Q *
      my_half g_root (p, o) * in_tree g g_root)
       |-- atomic_shift
-      (λ BST : tree, !! sorted_tree BST && tree_rep2 g g_root BST) ∅ ⊤
-      (λ (BST : tree) (ret : val),
-       !! (sorted_tree BST ∧ ret = lookup nullval x BST) &&
-       tree_rep2 g g_root BST * emp) Q * my_half g_root (p, o) *
+      (λ BST : tree, !! sorted_tree BST && tree_rep2 g g_root BST) ∅ ⊤ b Q *
+    my_half g_root (p, o) *
     (!! (p = (Neg_Infinity, Pos_Infinity)) && in_tree g g_root).
 Proof.
   intros. apply sync_rollback. intros t. Intros. unfold tree_rep2 at 1. Intros tg.
@@ -1773,17 +1826,14 @@ Proof.
 Qed.
 
 Lemma in_tree_left_range:
-  ∀ (x x0: Z) (g g_root : gname) (Q : val → mpred) (inv_names : invG) (v: val)
-    (g_in ga gb: gname) (r a: number * number * option ghost_info),
+  ∀ (B: Type) (b: tree -> B -> mpred) (Q : B → mpred) (x x0: Z) (g g_root : gname)
+    (inv_names : invG) (v: val) (g_in ga gb: gname)
+    (r a: number * number * option ghost_info),
     check_key_exist' x r.1 = true -> r.2 = Some (x0, v, ga, gb) -> x < x0 ->
     atomic_shift (λ BST : tree, !! sorted_tree BST && tree_rep2 g g_root BST) ∅ ⊤
-    (λ (BST : tree) (ret : val),
-     !! (sorted_tree BST ∧ ret = lookup nullval x BST) && tree_rep2 g g_root BST *
-     emp) Q * my_half g_in r * in_tree g g_in * my_half ga a
+                 b Q * my_half g_in r * in_tree g g_in * my_half ga a
     |-- atomic_shift (λ BST : tree, !! sorted_tree BST && tree_rep2 g g_root BST) ∅ ⊤
-    (λ (BST : tree) (ret : val),
-     !! (sorted_tree BST ∧ ret = lookup nullval x BST) && tree_rep2 g g_root BST *
-     emp) Q * my_half g_in r *
+    b Q * my_half g_in r *
     (!! (a.1 = (r.1.1, Finite_Integer x0)) && (in_tree g g_in * my_half ga a)).
 Proof.
   intros. rewrite sepcon_assoc. apply sync_rollback. intros t.
@@ -1809,17 +1859,14 @@ Proof.
 Qed.
 
 Lemma in_tree_right_range:
-  ∀ (x x0: Z) (g g_root : gname) (Q : val → mpred) (inv_names : invG) (v: val)
-    (g_in ga gb: gname) (r a: number * number * option ghost_info),
+  ∀ (B: Type) (b: tree -> B -> mpred) (Q : B → mpred) (x x0: Z) (g g_root : gname)
+    (inv_names : invG) (v: val) (g_in ga gb: gname)
+    (r a: number * number * option ghost_info),
     check_key_exist' x r.1 = true -> r.2 = Some (x0, v, ga, gb) -> x0 < x ->
     atomic_shift (λ BST : tree, !! sorted_tree BST && tree_rep2 g g_root BST) ∅ ⊤
-    (λ (BST : tree) (ret : val),
-     !! (sorted_tree BST ∧ ret = lookup nullval x BST) && tree_rep2 g g_root BST *
-     emp) Q * my_half g_in r * in_tree g g_in * my_half gb a
+                 b Q * my_half g_in r * in_tree g g_in * my_half gb a
     |-- atomic_shift (λ BST : tree, !! sorted_tree BST && tree_rep2 g g_root BST) ∅ ⊤
-    (λ (BST : tree) (ret : val),
-     !! (sorted_tree BST ∧ ret = lookup nullval x BST) && tree_rep2 g g_root BST *
-     emp) Q * my_half g_in r *
+    b Q * my_half g_in r *
     (!! (a.1 = (Finite_Integer x0, r.1.2)) && (in_tree g g_in * my_half gb a)).
 Proof.
   intros. rewrite sepcon_assoc. apply sync_rollback. intros t.
@@ -1860,7 +1907,12 @@ Proof.
   - (* current status implies lookup_inv *)
     unfold lookup_inv. Exists tp np (p, o) g_root lock.
     gather_SEP (atomic_shift _ _ _ _ _) (my_half _ _) (in_tree g _).
-    sep_apply (in_tree_root_range x g g_root Q inv_names p o). entailer. cancel.
+    sep_apply (in_tree_root_range
+                 val
+                 (λ (BST : tree) (ret : val),
+                  !! (sorted_tree BST ∧ ret = lookup nullval x BST) &&
+                  tree_rep2 g g_root BST * emp) Q g g_root inv_names p o).
+    entailer. cancel.
     unfold nodebox_rep. Exists np. cancel. unfold ltree, node_lock_inv. entailer!.
   - (* type check *) entailer!.
   - (* loop body *)
@@ -1879,7 +1931,11 @@ Proof.
       gather_SEP (atomic_shift _ _ _ _ _) (my_half g_in _)
                  (in_tree g g_in) (my_half ga a).
       sep_apply (in_tree_left_range
-                   x x0 g g_root Q inv_names v g_in ga gb r a). Intros.
+                   val
+                   (λ (BST : tree) (ret : val),
+                    !! (sorted_tree BST ∧ ret = lookup nullval x BST) &&
+                    tree_rep2 g g_root BST * emp)
+                   Q x x0 g g_root inv_names v g_in ga gb r a). Intros.
       forward_call (lock_in, lsh2, node_lock_inv_pred g np0 g_in lock_in,
                     node_lock_inv g np0 g_in lock_in). (* _release2(_l_old); *)
       * lock_props. setoid_rewrite node_lock_inv_def at 4. simpl. cancel.
@@ -1903,7 +1959,11 @@ Proof.
         gather_SEP (atomic_shift _ _ _ _ _) (my_half g_in _)
                    (in_tree g g_in) (my_half gb a).
         sep_apply (in_tree_right_range
-                     x x0 g g_root Q inv_names v g_in ga gb r a). Intros.
+                     val
+                     (λ (BST : tree) (ret : val),
+                      !! (sorted_tree BST ∧ ret = lookup nullval x BST) &&
+                      tree_rep2 g g_root BST * emp) Q
+                     x x0 g g_root inv_names v g_in ga gb r a). Intros.
         forward_call (lock_in, lsh2, node_lock_inv_pred g np0 g_in lock_in,
                       node_lock_inv g np0 g_in lock_in). (* _release2(_l_old__1); *)
         -- lock_props. setoid_rewrite node_lock_inv_def at 4. simpl. cancel.
@@ -2174,7 +2234,7 @@ Proof.
              iModIntro.  iPoseProof ( extract_lemmas_for_treerep2 with "[H1 H2]") as "Hadd". instantiate(1:= x0 ). auto. iFrame. iDestruct "Hadd" as (n1 n2 o0) "(H1 & H2)". 
              iExists (n1,n2,o0). iFrame. iPoseProof ( bi.and_elim_l with "H2") as "H3".  iPoseProof ( bi.and_elim_l with "H3") as "Hnew". iIntros "%". iDestruct "Hnew" as (g1 g2) "H".  iExists (n1,n2,Some(x,v,g1,g2)).  iIntros "(H1 & H2)".
              match goal with |-context[(|==> ?P)%logic] => change ((|==> P)%logic) with ((|==> P)%I) end. instantiate (1 := x). instantiate (1:= v). inv a.  iSpecialize ("H" with "[H2]"). iFrame. iSplit;auto. iMod "H". iModIntro. normalize. 
-             iExists g1. normalize.  iExists g2. iDestruct "H" as "(((((H2 & H3) & H4) & H5) & H6) & H7 )". apply (insert_sorted x v) in H7.  iFrame.  iSplit.  auto. auto. done.
+             iExists g1. normalize.  iExists g2. iDestruct "H" as "(((((H2 & H3) & H4) & H5) & H6) & H7 )". apply (insert_sorted x v) in H7.  iFrame.  iSplit.  auto. iFrame. done.
        }
       Intros g1 g2.
       forward_call (l1, Ews, (node_lock_inv g p1' g1 l1)).
